## Composition
If $f: X \to Y$ and $g:Y\to Z$  then $f;g:X\to Z$ is a function that is defined
- $f;g$ is sometimes written  $g \circ f$
- $(f;g)(x) = g(f(x))$
- $(g \circ f)(x) = f(g(x))$

![[Pasted image 20241102021337.png]]
## Associativity
Function composition is associative $(f;g);h = f;(g;h)$
Proof:
1. Setup
	- Let's consider three functions $f,g,h$
	- Let $x$ be any element in the domain of $h$
	- We need to show that $((f;g);h)(x) = (f;(g;h))(x)$
2. Let's Evaluate the left side: $((f;g);h)(x)$ 
	- By definition
		- $(f;g)(y)~\text{means}~ g(f(y))$
	- 